\subsection*{4-10}
\subsubsection*{(1)}
\begin{align}
  \begin{split}
    N&=\sum_{N=0}^\infty\sum_\nu\frac{1}{{\rm e}^{\beta(\varepsilon_\nu-\mu)}-1}\\
    &=\sum_{n_x}\sum_{n_y}\sum_{n_z}\frac{1}{{\rm e}^{\beta(\varepsilon_{\bm n}-\mu)}-1}\\
    &=\int_0^{\infty}{\rm d}{n_x}\int_0^{\infty}{\rm d}{n_y}\int_0^{\infty}{\rm d}{n_z}\frac{1}{{\rm e}^{\beta(\varepsilon_{\bm n}-\mu)}-1}
  \end{split}
\end{align}
ここで$\varepsilon_{\bm n}=\hbar\omega(n_x+n_y+n_z)$である.(定数部分は省略した)
\subsubsection*{(2)}
(23)式において$i=\beta\hbar\omega n_i\ (i=x,y,z)$すれば
\begin{align}
  \begin{split}
    N=\left(\frac{k_BT}{\hbar\omega}\right)^3\int_0^\infty{\rm d}x\int_0^\infty{\rm d}y\int_0^\infty{\rm d}z\frac{1}{{\rm e}^{-\beta\mu}{\rm e}^{x+y+z}-1}
  \end{split}
\end{align}
また
\begin{align}
  \begin{split}
    \int_0^\infty\frac{x^{n-1}}{z^{-1}{\rm e}^x-1}{\rm d}x&=\int_0^\infty\frac{x^{n-1}z{\rm e}^{-x}}{1-z{\rm e}^{-x}}\\
    &=\int_0^\infty x^{n-1}z{\rm e}^{-x}\sum_{k=0}^{\infty}{z{\rm e}^{-x}}^k{\rm d}x\\
    &=\sum_{k=0}^{\infty}\int_0^\infty t^{n-1}{\rm e}^{-t}{\rm d}t\frac{z^{k+1}}{(k+1)^n}\\
    &=\Gamma(n)\sum_{k=1}^\infty\frac{z^k}{k^n}
  \end{split}
\end{align}
を用いれば
\begin{align}
  \begin{split}
    N&=\left(\frac{k_BT_c}{\hbar\omega}\right)^3\int_0^\infty{\rm d}x\int_0^\infty{\rm d}y\ \Gamma(1)\sum_{k=1}^\infty\frac{{\rm e}^{-k(x+y-\beta\mu)}}{k}\\
    &=\left(\frac{k_BT_c}{\hbar\omega}\right)^3\int_0^\infty{\rm d}x\ \sum_{k=1}^\infty\frac{{\rm e}^{-k(x-\beta\mu)}}{k^{2}}\\
    &=\left(\frac{k_BT_c}{\hbar\omega}\right)^3\sum_{k=1}^\infty\frac{{\rm e}^{k\beta\mu}}{k^3}
  \end{split}
\end{align}
また$T\leq T_c$において$\mu=0$なので
\begin{align}
  N=\left(\frac{k_BT}{\hbar\omega}\right)^3\zeta(3)
\end{align}
したがって
\begin{align}
  T_c=\frac{\hbar\omega}{k_B}\left(\frac{N}{\zeta(3)}\right)^{1/3}
\end{align}
\subsubsection*{(3)}
(27)式は凝縮していない粒子の数なので,凝縮した粒子の数を$N_0(T)$とすると
\begin{align}
  N_0(T)=N-\left(\frac{k_BT}{\hbar\omega}\right)^3\zeta(3)
\end{align}
(28)式から$(k_B/\hbar\omega)^3\zeta(3)=N/T_c^3$なので
\begin{align}
  N_0(T)=N\left(1-\left(\frac{T}{T_c}\right)^3\right)
\end{align}